src/Lean/Meta/Tactic/Cases.lean
@@ -281,7 +281,7 @@ private def inductionCasesOn (mvarId : MVarId) (majorFVarId : FVarId) (givenName
   let casesOn := mkCasesOnName ctx.inductiveVal.name
   let ctors   := ctx.inductiveVal.ctors.toArray
   let s ← induction mvarId majorFVarId casesOn givenNames
-  pure $ toCasesSubgoals s ctors majorFVarId us params
+  return toCasesSubgoals s ctors majorFVarId us params
 
 def cases (mvarId : MVarId) (majorFVarId : FVarId) (givenNames : Array AltVarNames := #[]) : MetaM (Array CasesSubgoal) :=
   withMVarContext mvarId do
