src/Lean/Meta/Tactic/Subst.lean
@@ -14,7 +14,7 @@ import Lean.Meta.Tactic.FVarSubst
 
 namespace Lean.Meta
 
-def substCore (mvarId : MVarId) (hFVarId : FVarId) (symm := false) (fvarSubst : FVarSubst := {}) (clearH := true) : MetaM (FVarSubst × MVarId) :=
+def substCore (mvarId : MVarId) (hFVarId : FVarId) (symm := false) (fvarSubst : FVarSubst := {}) (clearH := true) (tryToSkip := false) : MetaM (FVarSubst × MVarId) :=
   withMVarContext mvarId do
     let tag ← getMVarTag mvarId
     checkNotAssigned mvarId `subst
@@ -44,7 +44,7 @@ def substCore (mvarId : MVarId) (hFVarId : FVarId) (symm := false) (fvarSubst : 
         let h       := mkFVar hFVarId
         /- Set skip to true if there is no local variable nor the target depend on the equality -/
         let skip ←
-          if vars.size != 2 then
+          if !tryToSkip || vars.size != 2 then
             pure false
           else
             let mvarType ← getMVarType mvarId
@@ -128,20 +128,20 @@ def subst (mvarId : MVarId) (hFVarId : FVarId) : MetaM MVarId :=
         let mvarId ← assert mvarId hLocalDecl.userName newType (mkFVar hFVarId)
         let (hFVarId', mvarId) ← intro1P mvarId
         let mvarId ← clear mvarId hFVarId
-        return (← substCore mvarId hFVarId' symm).2
+        return (← substCore mvarId hFVarId' (symm := symm) (tryToSkip := true)).2
       let rhs' ← whnf rhs
       if rhs'.isFVar then
         if rhs != rhs' then
           substReduced (← mkEq lhs rhs') true
         else
-          return (← substCore mvarId hFVarId true).2
+          return (← substCore mvarId hFVarId (symm := true) (tryToSkip := true)).2
       else do
         let lhs' ← whnf lhs
         if lhs'.isFVar then
           if lhs != lhs' then
             substReduced (← mkEq lhs' rhs) false
           else
-            return (← substCore mvarId hFVarId).2
+            return (← substCore mvarId hFVarId (symm := false) (tryToSkip := true)).2
         else do
           throwTacticEx `subst mvarId m!"invalid equality proof, it is not of the form (x = t) or (t = x){indentExpr hLocalDecl.type}"
     | none =>
@@ -163,7 +163,7 @@ def subst (mvarId : MVarId) (hFVarId : FVarId) : MetaM MVarId :=
                return none
            | _ => return none
         | throwTacticEx `subst mvarId m!"did not find equation for eliminating '{mkFVar hFVarId}'"
-      return (← substCore mvarId fvarId symm).2
+      return (← substCore mvarId fvarId (symm := symm) (tryToSkip := true)).2
 
 builtin_initialize registerTraceClass `Meta.Tactic.subst
 
