tests/lean/run/contradiction1.lean
@@ -1,0 +1,25 @@
+inductive MyFin : Nat → Type
+  | z : MyFin (n+1)
+  | s : MyFin n → MyFin (n+1)
+
+theorem ex1 (x : MyFin 0) : False := by
+  contradiction
+
+inductive Color
+| Red
+| Black
+open Color
+
+inductive rbnode : Nat → Color → Type where
+  | Leaf : rbnode 1 Black
+  | R {h}
+      (left : rbnode h Black)
+      (value : Int)
+      (right : rbnode h Black) : rbnode h Red
+  | B {h cl cr}
+      (left : rbnode h cl)
+      (value : Int)
+      (right : rbnode h cr) : rbnode (h+1) Black
+
+theorem ex2 (x : rbnode 0 Color.Red) : False := by
+  contradiction
